examples/Application.v
@@ -1,0 +1,12 @@
+(** * §6 Application *)
+
+(** ** §6.1 CompCertO Semantics *)
+Require Import CompCertStrat.
+(** ** §6.2 Memory Separation *)
+Require Import BQStrat.
+(** ** §6.3 Modeling loading and the execution environments *)
+Require Import Rot13.
+(** ** §6.4 Certified Abstraction Layers *)
+Require Import CALStrat.
+(** ** §6.5 ClightP *)
+Require Import ClightPStrat.
